\documentclass{article}
\usepackage{ifthen}
\usepackage{epsfig}
\usepackage[utf8]{inputenc}
\usepackage{newunicodechar}
  \newunicodechar{⁻}{${}^{-}$}% Superscript minus
  \newunicodechar{²}{${}^{2}$}% Superscript two
  \newunicodechar{³}{${}^{3}$}% Superscript three

\pagestyle{empty}
\begin{document}
\[ radius=\sqrt{(center_x-perimeter_x)^2+(center_y-perimeter_y)^2} \]
\pagebreak

\[ set_1 = set_1 \cup set_2 \]
\pagebreak

$\leq$
\pagebreak

\[ length=\sqrt{dx^2+dy^2} \]
\pagebreak

\[ length=\sqrt{(p2_x-p1_x)^2+(p2_y-p1_y)^2} \]
\pagebreak

\[ circumference=2*\pi*radius \]
\pagebreak

\[ angle=atan2(end_y-start_y, end_x-start_x) \]
\pagebreak

\[ distance=\sqrt{size_x^2+size_y^2} \]
\pagebreak

\[ area=size_w*size_h \]
\pagebreak

\[ area=\pi*radius^2 \]
\pagebreak

\[ \left[ \begin{array}{c} f_x \\ f_y \\ \end{array} \right] = \left[ \begin{array}{c} \log fsize_x \\ \log fsize_y \\ \end{array} \right] \]
\pagebreak

\[ \left[ \begin{array}{c} f_x \\ f_y \\ \end{array} \right] = \left[ \begin{array}{c} \lfloor fsize_x \\ \lfloor fsize_y \\ \end{array} \right] \]
\pagebreak

\[ \left[ \begin{array}{c} f_x \\ f_y \\ \end{array} \right] = \left[ \begin{array}{c} val \\ val \\ \end{array} \right] - \left[ \begin{array}{c} fsize_x \\ fsize_y \\ \end{array} \right] \]
\pagebreak

\[ \left[ \begin{array}{c} f_x \\ f_y \\ \end{array} \right] = \left[ \begin{array}{c} this_x \\ this_y \\ \end{array} \right] + \left[ \begin{array}{c} fsize_x \\ fsize_y \\ \end{array} \right] \]
\pagebreak

\[ \left[ \begin{array}{c} f_x \\ f_y \\ \end{array} \right] = \left[ \begin{array}{c} this_x \\ this_y \\ \end{array} \right] + \left[ \begin{array}{c} val \\ val \\ \end{array} \right] \]
\pagebreak

\[ \left[ \begin{array}{c} f_x \\ f_y \\ \end{array} \right] = \left[ \begin{array}{cc} this_x & 0 \\ 0 & this_y \\ \end{array} \right] \left[ \begin{array}{c} fsize_x \\ fsize_y \\ \end{array} \right] \]
\pagebreak

\[ \left[ \begin{array}{c} f_x \\ f_y \\ \end{array} \right] = \left[ \begin{array}{cc} this_x & 0 \\ 0 & this_y \\ \end{array} \right] \left[ \begin{array}{c} size_x \\ size_y \\ \end{array} \right] \]
\pagebreak

\[ \left[ \begin{array}{c} f_x \\ f_y \\ \end{array} \right] = mult \left[ \begin{array}{c} this_x \\ this_y \\ \end{array} \right] \]
\pagebreak

\[ \left[ \begin{array}{c} this_x \\ this_y \\ \end{array} \right] = \left[ \begin{array}{c} this_x \\ this_y \\ \end{array} \right] + \left[ \begin{array}{c} fsize_x \\ fsize_y \\ \end{array} \right] \]
\pagebreak

\[ \left[ \begin{array}{c} this_x \\ this_y \\ \end{array} \right] = \left[ \begin{array}{c} this_x \\ this_y \\ \end{array} \right] - \left[ \begin{array}{c} fsize_x \\ fsize_y \\ \end{array} \right] \]
\pagebreak

\[ \left[ \begin{array}{c} this_x \\ this_y \\ \end{array} \right] = \left[ \begin{array}{cc} this_x & 0 \\ 0 & this_y \\ \end{array} \right] \left[ \begin{array}{c} fsize_x \\ fsize_y \\ \end{array} \right] \]
\pagebreak

\end{document}
